scratch/AppIfPrimSpineUnsound.v
@@ -1,0 +1,312 @@
+From SymCoreTheory Require Import SymCore ConCore Model.
+From Stdlib Require Import Strings.String Lists.List Bool.Bool Arith.PeanoNat.
+Import ListNotations.
+
+Definition is_con (e : expr) : bool :=
+  match e with
+  | ECon _ => true
+  | _ => false
+  end.
+
+Fixpoint has_con_arg (e : expr) : bool :=
+  match e with
+  | EApp f a => is_con a || has_con_arg f
+  | _ => false
+  end.
+
+Definition result_con : dcon := "Result"%string.
+
+Definition answer_con_arg (e : expr) : expr :=
+  if has_con_arg e then ECon result_con else e.
+
+Fixpoint answer_leaves (e : expr) : expr :=
+  match e with
+  | EIf c t f => EIf c (answer_leaves t) (answer_leaves f)
+  | _ => answer_con_arg e
+  end.
+
+Definition con_reduce_prim (p : model_primop) (args : list expr) : expr :=
+  answer_leaves (model_reduce_prim p args).
+
+Definition con_solver : SymCoreSolver :=
+  Build_SymCoreSolver
+    model_sat (PCLit true) eq_refl con_reduce_prim
+    erase_cast keep_coercion keep_type.
+
+Lemma answer_leaves_not_if : forall e, is_if e = false -> answer_leaves e = answer_con_arg e.
+Proof. intros e H. destruct e; simpl in *; try reflexivity. discriminate. Qed.
+
+Lemma expr_to_pc_no_con_arg : forall Γ e pc,
+  expr_to_pc Γ e = Some pc -> has_con_arg e = false.
+Proof.
+  intros Γ e. induction e; intros pc H; simpl in *; try reflexivity.
+  destruct (expr_to_pc Γ e1) as [[| | p args]|] eqn:E1; try discriminate.
+  destruct (expr_to_pc Γ e2) as [pca|] eqn:E2; try discriminate.
+  rewrite (IHe1 _ eq_refl).
+  destruct e2; simpl in E2 |- *; try reflexivity. discriminate.
+Qed.
+
+Lemma answer_leaves_of_pc : forall Γ e pc,
+  expr_to_pc Γ e = Some pc -> answer_leaves e = e.
+Proof.
+  intros Γ e pc H.
+  assert (Hif : is_if e = false) by (destruct e; simpl in *; try reflexivity; discriminate).
+  rewrite (answer_leaves_not_if e Hif). unfold answer_con_arg.
+  rewrite (expr_to_pc_no_con_arg Γ e pc H). reflexivity.
+Qed.
+
+Lemma answer_leaves_of_denote : forall σ S e l, denote σ S e l -> answer_leaves e = e.
+Proof.
+  intros σ S e l [pc [Hd _]].
+  exact (answer_leaves_of_pc · e pc (Hd · (sym_free_env_empty S))).
+Qed.
+
+Lemma solvable_no_con_arg : forall Γ e, Solvable Γ e -> has_con_arg e = false.
+Proof.
+  intros Γ e H. induction H as [| | | f a Hop Hf IHf Ha IHa]; try reflexivity.
+  simpl. rewrite IHf. destruct a; inversion Ha; reflexivity.
+Qed.
+
+Lemma answer_leaves_of_solvable : forall Γ e, Solvable Γ e -> answer_leaves e = e.
+Proof.
+  intros Γ e H.
+  assert (Hif : is_if e = false) by (destruct H; reflexivity).
+  rewrite (answer_leaves_not_if e Hif). unfold answer_con_arg.
+  rewrite (solvable_no_con_arg Γ e H). reflexivity.
+Qed.
+
+Lemma contains_keeps_not_if : forall σ S es ec,
+  contains σ S es ec -> is_if es = false -> is_if ec = false.
+Proof. intros σ S es ec H Hif. destruct H; simpl in *; try reflexivity; discriminate. Qed.
+
+Lemma contains_keeps_is_con : forall σ S es ec,
+  contains σ S es ec -> is_if es = false -> is_con ec = is_con es.
+Proof.
+  intros σ S es ec H Hif. destruct H; simpl in *; try reflexivity; try discriminate.
+  match goal with
+  | [ Hu : unspool_app ?e _ = _, Hg : smt_ground ?e = false |- _ ] =>
+      destruct (cont_denote_is_app _ _ _ Hu Hg) as [? [? ->]]; reflexivity
+  end.
+Qed.
+
+Lemma contains_flat_con_arg : forall σ S es ec,
+  contains σ S es ec -> flat es = true -> has_con_arg ec = has_con_arg es.
+Proof.
+  intros σ S es ec H. induction H; intros Hflat; simpl in *; try reflexivity; try discriminate.
+  - apply andb_prop in Hflat as [Hf Ha].
+    rewrite (contains_keeps_is_con σ S a_s a_c H0 (flat_not_if a_s Ha)), (IHcontains1 Hf).
+    reflexivity.
+  - symmetry. destruct H2 as [pc [Hd _]].
+    exact (expr_to_pc_no_con_arg · es pc (Hd · (sym_free_env_empty S))).
+Qed.
+
+Lemma answer_con_arg_contains : forall σ S L X,
+  contains σ S L X -> flat L = true ->
+  contains σ S (answer_con_arg L) (answer_con_arg X).
+Proof.
+  intros σ S L X Hc Hf. unfold answer_con_arg.
+  rewrite (contains_flat_con_arg σ S L X Hc Hf).
+  destruct (has_con_arg L); [apply Cont_Con | exact Hc].
+Qed.
+
+Lemma picks_answer_leaves : forall σ S T L,
+  picks σ S T L -> picks σ S (answer_leaves T) (answer_con_arg L).
+Proof.
+  intros σ S T L H. induction H as [e Hif | c t f L Hm Hp IH | c t f L Hm Hp IH].
+  - rewrite (answer_leaves_not_if e Hif). apply picks_leaf.
+    unfold answer_con_arg. destruct (has_con_arg e); [reflexivity | exact Hif].
+  - apply picks_then; assumption.
+  - apply picks_else; assumption.
+Qed.
+
+Lemma flat_fold_leaf : forall L, flat L = true -> flat (fold_leaf L) = true.
+Proof. intros L H. unfold fold_leaf. destruct (smt_ground L); [reflexivity | exact H]. Qed.
+
+Instance con_reduce_prim_contains : @ReducePrimContains model_sorts con_solver.
+Proof.
+  intros σ S p args_s args_c HF.
+  change (contains σ S (con_reduce_prim p args_s) (con_reduce_prim p args_c)).
+  unfold con_reduce_prim, model_reduce_prim. rewrite <- (Forall2_length HF).
+  destruct (Nat.eqb (length args_s) (model_arity p)) eqn:Hlen; [| apply Cont_Lit].
+  apply Nat.eqb_eq in Hlen.
+  assert (Hc : contains σ S (op_spine p args_s) (op_spine p args_c))
+    by (apply contains_fold_left_app; [exact HF | apply Cont_PrimOp]).
+  rewrite (lift_flat _ (contains_flat_instance σ S _ _ Hc)),
+          (fold_leaves_not_if _ (op_spine_not_if p args_c)).
+  destruct (lift_picks σ S _ _ Hc) as [L [Hp [HcL HfL]]].
+  rewrite (answer_leaves_not_if _ (fold_leaf_not_if _ (op_spine_not_if p args_c))).
+  apply (picks_contains σ S _ (answer_con_arg (fold_leaf L)));
+    [apply picks_answer_leaves; apply picks_fold_leaves; exact Hp |].
+  apply answer_con_arg_contains; [| exact (flat_fold_leaf L HfL)].
+  apply (leaf_contains σ S p L); [| exact HcL | exact HfL].
+  rewrite <- Hlen. exact (picks_leaves σ S _ _ _ Hp (leaves_lift_spine p args_s)).
+Qed.
+
+Instance con_reduce_prim_denote : @ReducePrimDenote model_sorts con_solver.
+Proof.
+  intros σ S p args ls HF.
+  pose proof (@model_reduce_prim_denote σ S p args ls HF) as H.
+  change (denote σ S (model_reduce_prim p args) (prim_value p ls)) in H.
+  change (denote σ S (con_reduce_prim p args) (prim_value p ls)).
+  unfold con_reduce_prim. rewrite (answer_leaves_of_denote σ S _ _ H). exact H.
+Qed.
+
+Instance con_reduce_prim_ground_value : @ReducePrimGroundValue model_sorts con_solver.
+Proof.
+  intros p args H.
+  change (smt_ground (con_reduce_prim p args) = true) in H.
+  change (exists l, con_reduce_prim p args = ELit l).
+  unfold con_reduce_prim in *.
+  destruct (is_if (model_reduce_prim p args)) eqn:Hif.
+  - destruct (model_reduce_prim p args); simpl in Hif, H; discriminate.
+  - rewrite (answer_leaves_not_if _ Hif) in *. unfold answer_con_arg in *.
+    destruct (has_con_arg (model_reduce_prim p args)); [discriminate H |].
+    exact (@model_reduce_prim_ground_value p args H).
+Qed.
+
+Instance con_reduce_prim_saturated : @ReducePrimSaturated model_sorts con_solver.
+Proof.
+  intros p args p0 args0 H.
+  change (unspool_app (con_reduce_prim p args) nil = (EPrimOp p0, args0)) in H.
+  unfold con_reduce_prim in H.
+  destruct (is_if (model_reduce_prim p args)) eqn:Hif.
+  - destruct (model_reduce_prim p args); simpl in Hif, H; discriminate.
+  - rewrite (answer_leaves_not_if _ Hif) in H. unfold answer_con_arg in H.
+    destruct (has_con_arg (model_reduce_prim p args)); [discriminate H |].
+    exact (@model_reduce_prim_saturated p args p0 args0 H).
+Qed.
+
+Instance con_reduce_prim_solvable : @ReducePrimSolvable model_sorts con_solver.
+Proof.
+  intros Γ p args HF.
+  pose proof (@model_reduce_prim_solvable Γ p args HF) as H.
+  change (Solvable Γ (model_reduce_prim p args)) in H.
+  change (Solvable Γ (con_reduce_prim p args)).
+  unfold con_reduce_prim. rewrite (answer_leaves_of_solvable Γ _ H). exact H.
+Qed.
+
+Instance con_reduce_prim_concore : @ReducePrimConcore model_sorts con_solver.
+Proof.
+  intros p args HF.
+  pose proof (@model_reduce_prim_concore p args HF) as H.
+  change (concore_expr (model_reduce_prim p args)) in H.
+  change (concore_expr (con_reduce_prim p args)).
+  unfold con_reduce_prim.
+  rewrite (answer_leaves_not_if _ (concore_not_if _ H)). unfold answer_con_arg.
+  destruct (has_con_arg (model_reduce_prim p args)); [apply Con_Con | exact H].
+Qed.
+
+Instance con_reduce_prim_ite_contains : @ReducePrimIteContains model_sorts con_solver.
+Proof.
+  intros σ S ec et ef pt pf l Ht Hf Hc.
+  pose proof (@model_reduce_prim_ite_contains σ S ec et ef pt pf l Ht Hf Hc) as H.
+  change (contains σ S (model_reduce_prim op_ite (ec :: et :: ef :: nil)) (ELit l)) in H.
+  change (contains σ S (con_reduce_prim op_ite (ec :: et :: ef :: nil)) (ELit l)).
+  destruct (contains_if_inv σ S ec et ef (ELit l) Hc) as [[[pc [Hdc _]] _] | [[pc [Hdc _]] _]];
+  assert (Hden : denote σ S (model_reduce_prim op_ite (ec :: et :: ef :: nil))
+                   (prim_value op_ite (pc_value σ pc :: pc_value σ pt :: pc_value σ pf :: nil)))
+    by (apply (@model_reduce_prim_denote σ S op_ite);
+        apply Forall2_cons; [exists pc; split; [exact Hdc | reflexivity] |];
+        apply Forall2_cons; [exists pt; split; [exact Ht | reflexivity] |];
+        apply Forall2_cons; [exists pf; split; [exact Hf | reflexivity] |];
+        apply Forall2_nil);
+  unfold con_reduce_prim; rewrite (answer_leaves_of_denote σ S _ _ Hden); exact H.
+Qed.
+
+Instance con_laws : @ConCoreLaws model_sorts con_solver.
+Proof.
+  constructor.
+  - exact con_reduce_prim_solvable.
+  - exact con_reduce_prim_saturated.
+  - exact con_reduce_prim_concore.
+  - exact model_cast_expr_concore.
+  - exact model_models_sat.
+  - exact model_prim_value_and.
+  - exact con_reduce_prim_contains.
+  - exact con_reduce_prim_denote.
+  - exact con_reduce_prim_ground_value.
+  - exact con_reduce_prim_ite_contains.
+  - exact model_cast_expr_contains.
+  - exact model_subst_coerc_contains_env.
+  - exact model_subst_type_contains_env.
+Qed.
+
+Definition guard_var : var := "x"%string.
+Definition branch_operator : expr := EIf (EVar guard_var) (EPrimOp PNot) (EPrimOp PNot).
+Definition field_con : expr := ECon "D"%string.
+Definition symbolic_program : expr := EApp (EApp branch_operator field_con) (ELit true).
+Definition concrete_program : expr := EApp (EApp (EPrimOp PNot) field_con) (ELit true).
+Definition branch_symvars : symvars := fun y => String.eqb y guard_var.
+Definition branch_model : valuation := fun _ => true.
+
+Lemma negation_of_field_is_a_constructor :
+  con_reduce_prim PNot (field_con :: nil) = ECon result_con.
+Proof. reflexivity. Qed.
+
+Lemma symbolic_program_has_value :
+  exists v, @eval model_sorts con_solver Inf (PCLit true) · symbolic_program v.
+Proof.
+  eexists. unfold symbolic_program, branch_operator.
+  eapply (@Eval_AppSpine model_sorts con_solver).
+  - apply Comp_App. reflexivity.
+  - apply Eval_AppIf. eapply Eval_If.
+    + apply Eval_SymVar. reflexivity.
+    + reflexivity.
+    + eapply Eval_AppPrim; [reflexivity | reflexivity |].
+      apply Forall2_cons; [eapply Eval_Con; reflexivity | apply Forall2_nil].
+    + eapply Eval_AppPrim; [reflexivity | reflexivity |].
+      apply Forall2_cons; [eapply Eval_Con; reflexivity | apply Forall2_nil].
+  - change (@reduce_prim model_sorts con_solver PNot [make_con_app "D" (map (delay ·) [])])
+      with (ECon result_con).
+    apply Eval_AppIf. eapply Eval_If.
+    + apply Eval_SymVar. reflexivity.
+    + reflexivity.
+    + eapply Eval_Con. reflexivity.
+    + eapply Eval_Con. reflexivity.
+Qed.
+
+Lemma concrete_program_is_stuck :
+  forall v, ~ @eval model_sorts con_solver Inf (PCLit true) · concrete_program v.
+Proof.
+  intros v H. unfold concrete_program, field_con in H.
+  inversion H; subst.
+  - match goal with Hu : unspool_app _ _ = (ECon _, _) |- _ => simpl in Hu; discriminate Hu end.
+  - match goal with Hc : Comp _ _ |- _ => inversion Hc as [| | | | ? ? Hh]; simpl in Hh; discriminate Hh end.
+  - match goal with Hu : unspool_app _ _ = (EPrimOp _, _), Hl : length _ = _ |- _ =>
+      simpl in Hu; injection Hu as <- <-; simpl in Hl; discriminate Hl end.
+  - match goal with Hs : sat _ = false |- _ => discriminate Hs end.
+Qed.
+
+Lemma symbolic_program_contains_concrete_program :
+  contains branch_model branch_symvars symbolic_program concrete_program.
+Proof.
+  apply Cont_App; [apply Cont_App; [| apply Cont_Con] | apply Cont_Lit].
+  apply Cont_If_True; [| apply Cont_PrimOp].
+  exists (PCVar guard_var). split; [| reflexivity].
+  intros Γ Hfree. simpl. rewrite (Hfree guard_var eq_refl). reflexivity.
+Qed.
+
+Lemma concrete_program_concore : concore_expr concrete_program.
+Proof. repeat constructor. Qed.
+
+Theorem app_if_breaks_soundness :
+  ~ (forall Φ Γs Γc σ S e_sym e_con v_sym,
+       σ ⊨ Φ ->
+       contains_env σ S Γs Γc ->
+       contains σ S e_sym e_con ->
+       concore_expr e_con ->
+       @eval model_sorts con_solver Inf Φ Γs e_sym v_sym ->
+       exists v_con,
+         @eval model_sorts con_solver Inf (PCLit true) Γc e_con v_con /\
+         contains σ S v_sym v_con).
+Proof.
+  intros Hsound.
+  destruct symbolic_program_has_value as [v_sym Hv].
+  assert (Hm : @models model_sorts branch_model (PCLit true)) by reflexivity.
+  destruct (Hsound _ · · branch_model branch_symvars symbolic_program concrete_program
+              v_sym Hm (Cont_Env_Empty _ _) symbolic_program_contains_concrete_program
+              concrete_program_concore Hv) as [v_con [Hc _]].
+  exact (concrete_program_is_stuck v_con Hc).
+Qed.
+
+Print Assumptions app_if_breaks_soundness.
